theories/cast_calculus/typing.v
@@ -1,36 +1,108 @@
 From Autosubst Require Export Autosubst.
 From fae_gtlc_mu Require Export prelude.
 From fae_gtlc_mu.cast_calculus Require Export lang types consistency.standard.
+From Coq Require Import List.
 
-Reserved Notation "Γ ⊢ₜ e : τ" (at level 74, e, τ at next level).
+Reserved Notation "Γ & pΓ ⊢ₜ e : τ & pτ" (at level 74, pΓ, e, τ, pτ at next level).
 
-Definition Is_Closed (τ : type) := forall τ', τ.[τ'/] = τ.
-
-Inductive typed (Γ : list type) : expr → type → Prop :=
-  | Var_typed x τ : (Γ !! x = Some τ) → Γ ⊢ₜ Var x : τ
-  | Unit_typed : Γ ⊢ₜ Unit : TUnit
-  | Pair_typed e1 e2 τ1 τ2 :
-     Γ ⊢ₜ e1 : τ1 → Γ ⊢ₜ e2 : τ2 → Γ ⊢ₜ Pair e1 e2 : TProd τ1 τ2
-  | Fst_typed e τ1 τ2 : Γ ⊢ₜ e : TProd τ1 τ2 → Γ ⊢ₜ Fst e : τ1
-  | Snd_typed e τ1 τ2 : Γ ⊢ₜ e : TProd τ1 τ2 → Γ ⊢ₜ Snd e : τ2
-  | InjL_typed e τ1 τ2 : Γ ⊢ₜ e : τ1 → Γ ⊢ₜ InjL e : TSum τ1 τ2
-  | InjR_typed e τ1 τ2 : Γ ⊢ₜ e : τ2 → Γ ⊢ₜ InjR e : TSum τ1 τ2
-  | Case_typed e0 e1 e2 τ1 τ2 ρ :
-     Γ ⊢ₜ e0 : TSum τ1 τ2 → τ1 :: Γ ⊢ₜ e1 : ρ → τ2 :: Γ ⊢ₜ e2 : ρ →
-     Γ ⊢ₜ Case e0 e1 e2 : ρ
-  | Lam_typed e τ1 τ2 : τ1 :: Γ ⊢ₜ e : τ2 → Γ ⊢ₜ Lam e : TArrow τ1 τ2
-  | App_typed e1 e2 τ1 τ2 : Γ ⊢ₜ e1 : TArrow τ1 τ2 → Γ ⊢ₜ e2 : τ1 → Γ ⊢ₜ App e1 e2 : τ2
-  | Fold_typed e τ : Γ ⊢ₜ e : τ.[TRec τ/] → Γ ⊢ₜ Fold e : TRec τ
-  | Unfold_typed e τ : Γ ⊢ₜ e : TRec τ → Γ ⊢ₜ Unfold e : τ.[TRec τ/]
+Inductive typed (Γ : list type) (pΓ : Forall TClosed Γ) : expr → forall (τ : type), TClosed τ → Prop :=
+  | Var_typed x τ pτ : (Γ !! x = Some τ) → Γ & pΓ ⊢ₜ Var x : τ & pτ
+  | Unit_typed pu : (Γ & pΓ ⊢ₜ Unit : TUnit & pu)
+  | Pair_typed e1 e2 τ1 pτ1 τ2 pτ2 pτ12 :
+      Γ & pΓ ⊢ₜ e1 : τ1&pτ1 →
+      Γ & pΓ ⊢ₜ e2 : τ2&pτ2 →
+      Γ & pΓ ⊢ₜ Pair e1 e2 : TProd τ1 τ2 & pτ12
+  | Fst_typed e τ1 pτ1 τ2 pτ12 :
+      Γ & pΓ ⊢ₜ e : TProd τ1 τ2 & pτ12 →
+      Γ & pΓ ⊢ₜ Fst e : τ1 & pτ1
+  | Snd_typed e τ1 τ2 pτ2 pτ12 :
+      Γ & pΓ ⊢ₜ e : TProd τ1 τ2 & pτ12 →
+      Γ & pΓ ⊢ₜ Snd e : τ2 & pτ2
+  | InjL_typed e τ1 pτ1 τ2 pτ12 :
+      Γ & pΓ ⊢ₜ e : τ1&pτ1 →
+      Γ & pΓ ⊢ₜ InjL e : TSum τ1 τ2 & pτ12
+  | InjR_typed e τ1 τ2 pτ2 pτ12 :
+      Γ & pΓ ⊢ₜ e : τ2 & pτ2 →
+      Γ & pΓ ⊢ₜ InjR e : TSum τ1 τ2 & pτ12
+  | Case_typed e0 e1 e2 τ1 pτ1 τ2 pτ2 pτ12 τ pτ :
+      Γ & pΓ ⊢ₜ e0 : TSum τ1 τ2 & pτ12 →
+      τ1 :: Γ & (Forall_cons _ _ _ pτ1 pΓ) ⊢ₜ e1 : τ & pτ →
+      τ2 :: Γ & (Forall_cons _ _ _ pτ2 pΓ) ⊢ₜ e2 : τ & pτ →
+      Γ & pΓ ⊢ₜ Case e0 e1 e2 : τ & pτ
+  | Lam_typed e τ1 pτ1 τ2 pτ2 pτ12 :
+      τ1 :: Γ & (Forall_cons _ _ _ pτ1 pΓ) ⊢ₜ e : τ2 & pτ2 →
+      Γ & pΓ ⊢ₜ Lam e : TArrow τ1 τ2 & pτ12
+  | App_typed e1 e2 τ1 pτ1 τ2 pτ2 pτ12 :
+      Γ & pΓ ⊢ₜ e1 : TArrow τ1 τ2 & pτ12 →
+      Γ & pΓ ⊢ₜ e2 : τ1 & pτ1 →
+      Γ & pΓ ⊢ₜ App e1 e2 : τ2 & pτ2
+  | Fold_typed e τb pτbμτb pμτb :
+      Γ & pΓ ⊢ₜ e : τb.[TRec τb/] & pτbμτb →
+      Γ & pΓ ⊢ₜ Fold e : TRec τb & pμτb
+  | Unfold_typed e τb pμτb pτbμτb :
+      Γ & pΓ ⊢ₜ e : TRec τb & pμτb →
+      Γ & pΓ ⊢ₜ Unfold e : τb.[TRec τb/] & pτbμτb
   (* typing for CAST *)
-  | Cast_typed e τi τf : TClosed τi -> TClosed τf -> cons_stand τi τf → Γ ⊢ₜ e : τi → Γ ⊢ₜ Cast e τi τf : τf
+  | Cast_typed e τi pτi τf pτf (pC : cons_stand τi pτi τf pτf) :
+      Γ & pΓ ⊢ₜ e : τi & pτi →
+      Γ & pΓ ⊢ₜ Cast e τi τf : τf & pτf
   (* typing for BLAME *)
-  | Blame_typed τ : Is_Closed τ → Γ ⊢ₜ Blame : τ
+  | Blame_typed τ pτ :
+      Γ & pΓ ⊢ₜ Blame : τ & pτ
+where "Γ & pΓ ⊢ₜ e : τ & pτ" := (typed Γ pΓ e τ pτ).
   (* maybe adjust later to allow... *)
-where "Γ ⊢ₜ e : τ" := (typed Γ e τ).
 
-Lemma typed_subst_invariant Γ e τ s1 s2 :
-  Γ ⊢ₜ e : τ → (∀ x, x < length Γ → s1 x = s2 x) → e.[s1] = e.[s2].
+
+(* helper lemma's {{{ *)
+
+Lemma PI_typed Γ pΓ e τ pτ pτ' : Γ & pΓ ⊢ₜ e : τ & pτ → Γ & pΓ ⊢ₜ e : τ & pτ'.
+Proof. intro H. induction H; by econstructor. Qed.
+
+Lemma PI_Γ_typed Γ pΓ pΓ' e τ pτ : Γ & pΓ ⊢ₜ e : τ & pτ → Γ & pΓ' ⊢ₜ e : τ & pτ.
+Proof.
+  intro H. induction H; by econstructor.
+  Unshelve. auto. auto. auto.
+Qed.
+
+Lemma PI_Γ_typed' Γ pΓ' e τ pτ : forall pΓ, Γ & pΓ ⊢ₜ e : τ & pτ → Γ & pΓ' ⊢ₜ e : τ & pτ.
+Proof. intros pΓ H. by eapply PI_Γ_typed. Qed.
+
+Lemma Unfold_Fold_typed Γ pΓ e τ pτ :
+  Γ & pΓ ⊢ₜ e : τ & pτ → Γ & pΓ ⊢ₜ Unfold (Fold e) : τ & pτ.
+Proof.
+  intro.
+  assert (eq : τ = τ.[TRec τ/]). by rewrite pτ. generalize pτ. rewrite eq. intro pτμτ.
+  assert (pμτ : TClosed (TRec τ)). intro σ. asimpl. by rewrite pτ.
+  apply Unfold_typed with (pμτb := pμτ).
+  apply Fold_typed with (pτbμτb := pτμτ).
+  generalize pτμτ. rewrite -eq. intro pτ'.
+  by eapply PI_typed.
+Qed.
+
+Lemma Unfold_typed_help Γ pΓ e τb μτb τ' pτ' : (τb.[TRec τb/] = τ') →
+  Γ & pΓ ⊢ₜ e : (TRec τb) & μτb →
+  Γ & pΓ ⊢ₜ Unfold e : τ' & pτ'.
+Proof.
+  intros eq d.
+  generalize pτ'. rewrite -eq. intro pτ. eapply Unfold_typed.
+  by eapply PI_typed.
+  Unshelve. auto.
+Qed.
+
+Lemma rewrite_typed {Γ pΓ e τ pτ τ' pτ'} :
+  Γ & pΓ ⊢ₜ e : τ & pτ → τ = τ' → Γ & pΓ ⊢ₜ e : τ' & pτ'.
+Proof.
+  intros P eq.
+  generalize pτ'. rewrite -eq.
+  intro. by eapply PI_typed.
+Qed.
+
+(* }}} *)
+
+(* lemma's about substs in terms {{{ *)
+
+Lemma typed_subst_invariant Γ pΓ e τ pτ s1 s2 :
+  Γ & pΓ ⊢ₜ e : τ & pτ → (∀ x, x < length Γ → s1 x = s2 x) → e.[s1] = e.[s2].
 Proof.
   intros Htyped; revert s1 s2.
   assert (∀ x Γ, x < length (subst (ren (+1)) <$> Γ) → x < length Γ).
@@ -57,22 +129,10 @@ Proof.
     apply IHx.
 Qed.
 
-Lemma typed_n_closed Γ τ e : Γ ⊢ₜ e : τ → (∀ f, e.[upn (length Γ) f] = e).
+Lemma typed_n_closed Γ pΓ τ pτ e : Γ & pΓ ⊢ₜ e : τ & pτ → (∀ f, e.[upn (length Γ) f] = e).
 Proof.
   intros H. induction H => f; asimpl; simpl in *; auto with f_equal.
   apply lookup_lt_Some in H. rewrite iter_up. destruct lt_dec; auto with lia.
-Qed.
-
-Lemma Unfold_typed_help Γ e τ : (τ.[TRec τ/] = τ) → Γ ⊢ₜ e : TRec τ → Γ ⊢ₜ Unfold e : τ.
-Proof.
-  intros eq d.
-  rewrite -eq. by apply Unfold_typed.
-Qed.
-
-Lemma Unfold_typed_help_2 Γ e τ τ' : (τ.[TRec τ/] = τ') → Γ ⊢ₜ e : TRec τ → Γ ⊢ₜ Unfold e : τ'.
-Proof.
-  intros eq d.
-  rewrite -eq. by apply Unfold_typed.
 Qed.
 
 Lemma n_closed_invariant n (e : expr) s1 s2 :
@@ -109,33 +169,53 @@ Proof.
 Qed.
 
 (** Weakening *)
-Lemma context_gen_weakening ξ Γ' Γ e τ :
-  Γ' ++ Γ ⊢ₜ e : τ →
-  Γ' ++ ξ ++ Γ ⊢ₜ e.[upn (length Γ') (ren (+ (length ξ)))] : τ.
+Lemma context_gen_weakening ξ Γ' Γ α β e τ pτ :
+  Γ' ++ Γ & α ⊢ₜ e : τ & pτ →
+  Γ' ++ ξ ++ Γ & β ⊢ₜ e.[upn (length Γ') (ren (+ (length ξ)))] : τ & pτ.
 Proof.
   intros H1.
-  remember (Γ' ++ Γ) as Ξ. revert Γ' Γ ξ HeqΞ.
+  remember (Γ' ++ Γ) as Ξ. revert β. revert Γ' Γ ξ HeqΞ.
   induction H1 => Γ1 Γ2 ξ HeqΞ; subst; asimpl in *; eauto using typed.
   - rewrite iter_up; destruct lt_dec as [Hl | Hl].
-    + constructor. rewrite lookup_app_l; trivial. by rewrite lookup_app_l in H.
-    + asimpl. constructor. rewrite lookup_app_r; auto with lia.
+    + eapply Var_typed. rewrite lookup_app_l; trivial. by rewrite lookup_app_l in H.
+    + asimpl. eapply Var_typed. rewrite lookup_app_r; auto with lia.
       rewrite lookup_app_r; auto with lia.
       rewrite lookup_app_r in H; auto with lia.
       match goal with
         |- _ !! ?A = _ => by replace A with (x - length Γ1) by lia
       end.
   - econstructor; eauto. by apply (IHtyped2 (_::_)). by apply (IHtyped3 (_::_)).
-  - constructor. by apply (IHtyped (_ :: _)).
+  - eapply Lam_typed. by apply (IHtyped (_ :: _)).
+    Unshelve. auto. auto. auto.
 Qed.
 
-Lemma context_weakening ξ Γ e τ :
-  Γ ⊢ₜ e : τ → ξ ++ Γ ⊢ₜ e.[(ren (+ (length ξ)))] : τ.
+Lemma context_weakening ξ Γ pΓ α e τ pτ :
+  Γ & pΓ ⊢ₜ e : τ & pτ → ξ ++ Γ & α ⊢ₜ e.[(ren (+ (length ξ)))] : τ & pτ.
 Proof. eapply (context_gen_weakening _ []). Qed.
 
-(* Lemma context_gen_reorder Γ'' Γ' Γ τ1 τ2 τe τ : *)
-  (* Γ'' ++ [τ1] ++ Γ' ++ [τ2] ++ Γ ⊢ₜ e : τ → *)
-  (* Γ'' ++ [τ2] ++ Γ' ++ [τ1] ++ Γ' ⊢ₜ e.[upn (length Γ') (ren (+ (length ξ)))] : τ. *)
+Lemma up_type i Γ pΓ e τ pτ Γ' α : (length Γ' = i) -> (Γ & pΓ ⊢ₜ e : τ & pτ) -> (Γ' ++ Γ) & α ⊢ₜ e.[ren (+i)] : τ & pτ.
+Proof.
+  intros.
+  simplify_eq.
+  by eapply context_weakening.
+Qed.
 
-Lemma closed_context_weakening ξ Γ e τ :
-  (∀ f, e.[f] = e) → Γ ⊢ₜ e : τ → ξ ++ Γ ⊢ₜ e : τ.
-Proof. intros H1 H2. erewrite <- H1. by eapply context_weakening. Qed.
+Lemma up_type_one Γ pΓ e τ pτ τ' pτ' :
+  (Γ & pΓ ⊢ₜ e : τ & pτ) ->
+  ((τ' :: Γ) & (List.Forall_cons TClosed _ _ pτ' pΓ) ⊢ₜ e.[ren (+1)] : τ & pτ).
+Proof.
+  intro.
+  assert (T : τ' :: Γ = [τ'] ++ Γ). done. generalize (Forall_cons TClosed τ' Γ pτ' pΓ). rewrite T. intro α'.
+  by eapply up_type.
+Qed.
+
+Lemma up_type_two Γ pΓ e τ pτ τ' τ'' α :
+  (Γ & pΓ ⊢ₜ e : τ & pτ) ->
+  τ' :: τ'' :: Γ & α ⊢ₜ e.[ren (+2)] : τ & pτ.
+Proof.
+  intros.
+  assert (T : τ' :: τ'' :: Γ = [τ' ; τ''] ++ Γ). done. generalize α. rewrite T. intro.
+  by eapply up_type.
+Qed.
+
+(* }}} *)
