theories/refinements/static_gradual/logical_relation.v
@@ -5,18 +5,11 @@ From fae_gtlc_mu.backtranslation.cast_help Require Export embed.
 From fae_gtlc_mu.refinements Require Export prelude.
 From fae_gtlc_mu.refinements.static_gradual Require Export resources_left resources_right.
 From fae_gtlc_mu.cast_calculus Require Export types.
-From iris.algebra Require Import list.
+From iris.algebra Require Import list ofe.
 From stdpp Require Import tactics.
 Import uPred.
 
-(* Definition exprO := stlc_mu.lang.expr. *)
-(* Definition exprO' := cast_calculus.lang.expr. *)
-
-(* Definition valO := stlc_mu.lang.valO. *)
-(* Definition valO' := cast_calculus.lang.valO'. *)
-
-(* Coercion stlc_mu.lang.of_val : stlc_mu.lang.val >-> stlc_mu.lang.expr. *)
-(* Coercion cast_calculus.lang.of_val : cast_calculus.lang.val >-> cast_calculus.lang.expr. *)
+Canonical Structure typeO := leibnizO type.
 
 (* HACK: move somewhere else *)
 Ltac auto_equiv :=
@@ -37,334 +30,169 @@ Definition logN : namespace := nroot .@ "logN".
 (** interp : is a binary logical relation. *)
 Section logrel.
   Context `{!implG Σ, !specG Σ}.
+  Notation P := (prodO stlc_mu.lang.valO cast_calculus.lang.valO).
   Notation D := (prodO stlc_mu.lang.valO cast_calculus.lang.valO -n> iPropO Σ).
   Implicit Types τi : D.
   Implicit Types Δ : listO D.
-  (* Implicit Types interp : listO D → D. *)
-  Notation RelV := (listO D -n> D). (* value relation on (open) types *)
-
-  (* we get Initially from definition in fundamental_binary *)
-
-  Definition interp_expr (interp_cor_val : RelV) (Δ : listO D)
-      (ee : stlc_mu.lang.expr * cast_calculus.lang.expr) : iProp Σ := (∀ K',
-    currently_half (fill K' (ee.2)) →
-    WP ee.1 {{ v, ∃ v', currently_half (fill K' (of_val v')) ∗ interp_cor_val Δ (v, v') }})%I.
-  Global Instance interp_expr_ne n :
-    Proper (dist n ==> dist n ==> (=) ==> dist n) interp_expr.
-  Proof. solve_proper. Qed.
-
-  Program Definition ctx_lookup (x : var) : RelV := λne Δ,
-    from_option id (cconst True)%I (Δ !! x).
-  (* defaults to something which is trivially true if not in scope; OK, this will never happen in actual type derivations *)
-  Solve Obligations with solve_proper.
-
-  (** For the recursive call to structurally smaller types,
-      we will use the names interp, interp1, interp2... *)
-
-  Program Definition interp_unit : RelV := λne Δ ww,
-    (⌜ww.1 = stlc_mu.lang.UnitV⌝ ∧ ⌜ww.2 = cast_calculus.lang.UnitV⌝)%I.
-  Solve Obligations with solve_proper_alt.
-
-  Program Definition interp_sum
-      (interp1 interp2 : RelV) : RelV := λne Δ ww,
-    ((∃ vv', ⌜ww = (stlc_mu.lang.InjLV (vv'.1), InjLV (vv'.2))⌝ ∧ interp1 Δ vv') ∨
-     (∃ vv', ⌜ww = (stlc_mu.lang.InjRV (vv'.1), InjRV (vv'.2))⌝ ∧ interp2 Δ vv'))%I.
-  Solve Obligations with repeat intros ?; simpl; auto_equiv.
-
-  Program Definition interp_prod
-      (interp1 interp2 : RelV) : RelV := λne Δ ww,
-    (∃ v1v1' v2v2', ⌜ww = (stlc_mu.lang.PairV (v1v1'.1) (v2v2'.1), cast_calculus.lang.PairV (v1v1'.2) (v2v2'.2))⌝ ∧
-                interp1 Δ v1v1' ∧ interp2 Δ v2v2')%I.
-  Solve Obligations with repeat intros ?; simpl; auto_equiv.
-
-  Program Definition interp_arrow
-      (interp1 interp2 : RelV) : RelV := λne Δ ww,
-    (□ ∀ vv, interp1 Δ vv →
-             interp_expr
-               interp2 Δ (stlc_mu.lang.App (stlc_mu.lang.of_val (ww.1)) (stlc_mu.lang.of_val (vv.1)),
-                          cast_calculus.lang.App (cast_calculus.lang.of_val (ww.2)) (cast_calculus.lang.of_val (vv.2))))%I.
-  Solve Obligations with repeat intros ?; simpl; auto_equiv.
-
-  Program Definition interp_rec1 (* interp_rec1 interp Δ : D → D *)
-      (interp : RelV) (Δ : listO D) (μ : D) : D := λne ww,
-    (□ ∃ vv, ⌜ww = (stlc_mu.lang.FoldV (vv.1), cast_calculus.lang.FoldV (vv.2))⌝ ∧ ▷ interp (μ :: Δ) vv)%I.
-  Solve Obligations with repeat intros ?; simpl; auto_equiv.
-
-  Global Instance interp_rec1_contractive
-    (interp : listO D -n> D) (Δ : listO D) : Contractive (interp_rec1 interp Δ).
-  Proof. by solve_contractive. Qed.
-
-  Lemma fixpoint_interp_rec1_eq (interp : RelV) Δ x :
-    fixpoint (interp_rec1 interp Δ) x ≡ interp_rec1 interp Δ (fixpoint (interp_rec1 interp Δ)) x.
-  Proof. exact: (fixpoint_unfold (interp_rec1 interp Δ) x). Qed.
-
-  Lemma fixpoint_interp_rec1_eq2 (interp : RelV) Δ :
-    fixpoint (interp_rec1 interp Δ) ≡ interp_rec1 interp Δ (fixpoint (interp_rec1 interp Δ)).
-  Proof. exact: (fixpoint_unfold (interp_rec1 interp Δ)). Qed.
-
-  (* Definition interp_rec (interp : RelV) Δ : D := *)
-  (*   fixpoint (interp_rec1 interp Δ). *)
-
-  (* Global Instance interp_rec_ne n : Proper (dist (A := RelV) n ==> dist (A := RelV) n) interp_rec. *)
-
-
-  Program Definition interp_rec (interp : RelV) : RelV := λne Δ,
-    fixpoint (interp_rec1 interp Δ).
-  Next Obligation.
-    intros interp n Δ1 Δ2 HΔ; apply fixpoint_ne => τi ww. solve_proper.
-  Qed.
-
-  Global Instance interp_rec_ne n : Proper (dist n ==> dist n) interp_rec.
-  Proof.
-    repeat intros ?.
-    rewrite /interp_rec /=. apply (fixpoint_ne (interp_rec1 _ _)).
-    repeat intros ?. unfold interp_rec1.
-    simpl.
-    auto_equiv.
-  Qed.
-
-  (* Unset Printing Notations. *)
-  (* Set Printing Implicit. *)
-  (* Set Printing Notations. *)
-  (* Set Printing Coercions. *)
-
-  (* Unset Printing Notations. *)
-
-
-  (* Set Printing Implicit. *)
-  (* Unset Printing Implicit. *)
-
-  (* Set Printing All. *)
 
   Definition castupV_TUnit (v : val) : val :=
-    (CastV v TUnit ⋆ (From_ground_to_unknown _ Ground_TUnit)).
+    (CastV v TUnit ⋆ (TGround_TUnknown_icp Ground_TUnit)).
 
   Definition castupV_TSum (v : val) : val :=
-    (CastV v (TSum ⋆ ⋆) ⋆ (From_ground_to_unknown _ Ground_TSum)).
+    (CastV v (TSum ⋆ ⋆) ⋆ (TGround_TUnknown_icp Ground_TSum)).
 
   Definition castupV_TProd (v : val) : val :=
-    (CastV v (TProd ⋆ ⋆) ⋆ (From_ground_to_unknown _ Ground_TProd)).
+    (CastV v (TProd ⋆ ⋆) ⋆ (TGround_TUnknown_icp Ground_TProd)).
 
   Definition castupV_TArrow (v : val) : val :=
-    (CastV v (TArrow ⋆ ⋆) ⋆ (From_ground_to_unknown _ Ground_TArrow)).
+    (CastV v (TArrow ⋆ ⋆) ⋆ (TGround_TUnknown_icp Ground_TArrow)).
 
   Definition castupV_TRec (v : val) : val :=
-    (CastV v (TRec ⋆) ⋆ (From_ground_to_unknown _ Ground_TRec)).
+    (CastV v (TRec ⋆) ⋆ (TGround_TUnknown_icp Ground_TRec)).
 
-  (* interp_unknown1 : RelV -n> RelV *)
-  (* Program Definition interp_unknown1 : RelV -n> RelV := λne μR Δ ww', *)
-  Program Definition interp_unknown1 : RelV -n> RelV := λne μR Δ ww',
-   (□ (
-          (∃ vv', ⌜ ww' = (embedV_TUnit (vv'.1) , castupV_TUnit vv'.2) ⌝ ∧
-                ▷ interp_unit Δ vv' )
-        ∨ (∃ pp', ⌜ ww' = (embedV_Ground_TProd (pp'.1) , castupV_TProd pp'.2) ⌝ ∧
-                  ▷ interp_prod μR μR Δ pp')
-        ∨ (∃ ss', ⌜ ww' = (embedV_Ground_TSum (ss'.1) , castupV_TSum ss'.2) ⌝ ∧
-                  ▷ interp_sum μR μR Δ ss' )
-        ∨ (∃ ff', ⌜ ww' = (embedV_Ground_TArrow (ff'.1) , castupV_TArrow ff'.2) ⌝ ∧
-                  ▷ interp_arrow μR μR Δ ff' )
-        ∨ (∃ ur', ⌜ ww' = (stlc_mu.lang.FoldV (stlc_mu.lang.InjRV (ur'.1)) , castupV_TRec ur'.2) ⌝ ∧
-                  ▷ interp_rec μR Δ (stlc_mu.lang.FoldV ur'.1 , ur'.2))
+  Definition interp_expr (interp_cor_val : P → iPropO Σ)
+      (ee : stlc_mu.lang.expr * cast_calculus.lang.expr) : iProp Σ := (∀ K',
+    currently_half (fill K' (ee.2)) →
+    WP ee.1 {{ v, ∃ v', currently_half (fill K' (of_val v')) ∗ interp_cor_val (v, v') }})%I.
+
+  Definition TClosed (τ : type) : Prop := forall σ, τ.[σ] = τ.
+
+  (** only to be used with closed types *)
+
+  Fixpoint interp_gen (Ψ : typeO -n> D) (τ : typeO) (ww : P) : iPropO Σ := (
+    match τ with
+    | TUnit => ⌜ww.1 = stlc_mu.lang.UnitV⌝ ∧ ⌜ww.2 = cast_calculus.lang.UnitV⌝
+    | TProd τ1 τ2 => ∃ v1v1' v2v2', ⌜ww = (stlc_mu.lang.PairV (v1v1'.1) (v2v2'.1), cast_calculus.lang.PairV (v1v1'.2) (v2v2'.2))⌝ ∧
+                                  interp_gen Ψ τ1 v1v1' ∧ interp_gen Ψ τ2 v2v2'
+    | TSum τ1 τ2 => (∃ vv', ⌜ww = (stlc_mu.lang.InjLV (vv'.1), InjLV (vv'.2))⌝ ∧ interp_gen Ψ τ1 vv') ∨
+                    (∃ vv', ⌜ww = (stlc_mu.lang.InjRV (vv'.1), InjRV (vv'.2))⌝ ∧ interp_gen Ψ τ2 vv')
+    | TArrow τ1 τ2 => □ ∀ vv, interp_gen Ψ τ1 vv →
+             interp_expr
+               (interp_gen Ψ τ2) (stlc_mu.lang.App (stlc_mu.lang.of_val (ww.1)) (stlc_mu.lang.of_val (vv.1)),
+                        cast_calculus.lang.App (cast_calculus.lang.of_val (ww.2)) (cast_calculus.lang.of_val (vv.2)))
+    | TRec τb => □ ∃ w w', ⌜ww = (stlc_mu.lang.FoldV w, cast_calculus.lang.FoldV w')⌝ ∧ ▷ Ψ (τb.[TRec τb/]) (w, w')
+    | TUnknown => ∃ v v', □ (
+                               (⌜ ww = (embedV_TUnit v , castupV_TUnit v') ⌝                   ∧ ▷ Ψ TUnit (v, v') )
+                             ∨ (⌜ ww = (embedV_Ground_TProd v , castupV_TProd v') ⌝            ∧ ▷ Ψ (TProd TUnknown TUnknown) (v , v'))
+                             ∨ (⌜ ww = (embedV_Ground_TSum v , castupV_TSum v') ⌝              ∧ ▷ Ψ (TSum TUnknown TUnknown) (v , v'))
+                             ∨ (⌜ ww = (embedV_Ground_TArrow v , castupV_TArrow v') ⌝          ∧ ▷ Ψ (TArrow TUnknown TUnknown) (v , v'))
+                             ∨ (∃ u u', ⌜ ww = (embedV_TUnknown u, castupV_TRec (FoldV u')) ⌝ ∧ ▷ Ψ TUnknown (u , u')
+                               )
       )
-   )%I.
-  Next Obligation.
-    repeat intros ?; simpl; auto_equiv.
-  Qed.
-  Next Obligation.
-    repeat intros ?.  simpl; auto_equiv.
-    change (interp_rec μR x ≡{n}≡ interp_rec μR y). (*note*)
-    by f_equiv.
-  Qed.
-  Next Obligation.
-    repeat intros ?; simpl; auto_equiv.
-    change (interp_rec x x0 ≡{n}≡ interp_rec y x0). (*not use autogenerated names*)
-    f_equiv. by f_equiv.
-  Qed.
+    | TVar x => False (** exfaslo ... *)
+    end)%I.
 
-  Global Instance interp_unknown1_contractive : Contractive (interp_unknown1).
-  Proof.
-    repeat intros ?.
-    unfold interp_unknown1.
-    simpl. do 1 f_equiv.
-    repeat (f_equiv; first solve_contractive).
-    f_equiv. simpl. repeat intros ?.
-    f_equiv. f_equiv. intros ?. f_equiv. apply later_contractive.
-    destruct n; first done.
-    simpl in *. f_equiv.
-    intros ?. f_equiv. intros ?. by repeat f_equiv.
-
-    f_equiv. f_equiv. intros ?. f_equiv. apply later_contractive. destruct n; first done. simpl in *. by repeat f_equiv.
-    f_equiv. f_equiv. intros ?. f_equiv. apply later_contractive. destruct n; first done. simpl in *. by repeat f_equiv.
-    f_equiv. intros ?. f_equiv. apply later_contractive. destruct n; first done. simpl in *.
-    f_equiv.
-    change (interp_rec x x0 ≡{n}≡ interp_rec y x0). (*not use autogenerated names*)
-    by do 2 f_equiv.
-  Qed.
-
-  (* Global Instance interp_unknown1_contractive : Contractive (interp_unknown1). *)
-  (* Proof. *)
-  (*   repeat intros ?. *)
-  (*   unfold interp_unknown1. *)
-  (*   simpl. do 1 f_equiv. *)
-  (*   repeat (f_equiv; first solve_contractive). *)
-  (*   f_equiv. simpl. repeat intros ?. *)
-  (*   f_equiv. apply later_contractive. *)
-  (*   destruct n; first done. *)
-  (*   simpl in *. f_equiv. *)
-  (*   change (interp_rec x x0 ≡{n}≡ interp_rec y x0). (*not use autogenerated names*) *)
-  (*   by do 2 f_equiv. *)
-  (* Qed. *)
-
-  Definition interp_unknown : listO D -n> D := fixpoint (interp_unknown1).
-
-  Lemma interp_unknown_unfold Δ vv : interp_unknown Δ vv ≡ interp_unknown1 (fixpoint interp_unknown1) Δ vv.
-  Proof.
-    f_equiv.
-    f_equiv.
-    apply fixpoint_unfold.
-  Qed.
-
-  Lemma interp_unknown_unfold' Δ : interp_unknown Δ ≡ interp_unknown1 (fixpoint interp_unknown1) Δ.
-  Proof.
-    f_equiv.
-    apply fixpoint_unfold.
-  Qed.
-
-  (** Redefine it so it is more trivially contractive and independent from Δ *)
-  (** Also do some unfolding in the meantime..; will make it easier *)
-  Program Definition interp_unknown1' : D -n> D := λne μRc ww',
-   (□ (
-        (⌜ ww' = (embedV_TUnit (stlc_mu.lang.UnitV) , castupV_TUnit UnitV) ⌝)
-
-      ∨ (∃ v1 v1' v2 v2', ⌜ ww' = (embedV_Ground_TProd (stlc_mu.lang.PairV v1 v2) , castupV_TProd (PairV v1' v2')) ⌝ ∧ (▷ μRc (v1, v1')) ∧ (▷ μRc (v2, v2'))
-        )
-
-      ∨ ((∃ v1 v1', ⌜ ww' = (embedV_Ground_TSum (stlc_mu.lang.InjLV v1) , castupV_TSum (InjLV v1')) ⌝ ∧ ▷ μRc (v1 , v1')) ∨
-         (∃ v2 v2', ⌜ ww' = (embedV_Ground_TSum (stlc_mu.lang.InjRV v2) , castupV_TSum (InjRV v2')) ⌝ ∧ ▷ μRc (v2 , v2'))
-        )
-      ∨ (∃ f f', ⌜ ww' = (embedV_Ground_TArrow f , castupV_TArrow f') ⌝ ∧
-                ▷ □ ( ∀ a  a', μRc (a , a') →
-                             ∀ K', currently_half (fill K' (App f' a')) → WP (f a) {{ v , ∃ v', currently_half (fill K' (# v')) ∗ μRc (v , v') }} )
-        )
-      ∨ (∃ u u', ⌜ ww' = (stlc_mu.lang.FoldV (stlc_mu.lang.InjRV (u)) , castupV_TRec (FoldV u')) ⌝ ∧
-                ▷ μRc (u , u')
-        )
-      )
-   )%I.
+  Program Definition interp_gen_ne (Ψ : typeO -n> D) : typeO -n> D := λne τ p, interp_gen Ψ τ p.
   Solve Obligations with repeat intros ?; simpl; auto_equiv.
 
-  Global Instance interp_unknown1'_contractive : Contractive (interp_unknown1').
-  Proof. by solve_contractive. Qed.
-
-  Definition interp_unknown_pre' : D := fixpoint (interp_unknown1').
-
-  Lemma unfold_fixpoint_interp_unknown1' Δ vv : fixpoint interp_unknown1' vv ≡ interp_unknown1' (fixpoint interp_unknown1') vv.
+  Global Instance interp_gen_ne_contractive : Contractive interp_gen_ne.
   Proof.
-    f_equiv; apply fixpoint_unfold.
+    intros n Ψ1 Ψ2  pnΨ τ. simpl.
+    induction τ; intro p; simpl.
+    - auto.
+    - f_equiv. intro p1. f_equiv. intro p2. f_equiv. f_equiv.
+      + exact (IHτ1 p1).
+      + exact (IHτ2 p2).
+    - f_equiv.
+      + f_equiv. intro a. f_equiv. exact (IHτ1 a).
+      + f_equiv. intro a. f_equiv. exact (IHτ2 a).
+    - f_equiv. f_equiv. intro. f_equiv.
+      + exact (IHτ1 a).
+      + rewrite /interp_expr. simpl. f_equiv. intro K.
+        f_equiv. f_equiv. intro v. f_equiv. intro v'.
+        f_equiv. exact (IHτ2 (v, v')).
+    - solve_contractive.
+    - solve_contractive.
+    - solve_contractive.
   Qed.
 
-  Program Definition interp_unknown' : listO D -n> D := λne Δ vv, (interp_unknown_pre' vv)%I.
-  Solve Obligations with repeat intros ?; simpl; auto_equiv.
+  Definition interp : typeO -n> D := fixpoint interp_gen_ne.
 
-  Fixpoint interp (τ : cast_calculus.types.type) : listO D -n> D :=
-    match τ return _ with
-    | TUnit => interp_unit
-    | TProd τ1 τ2 => interp_prod (interp τ1) (interp τ2)
-    | TSum τ1 τ2 => interp_sum (interp τ1) (interp τ2)
-    | TArrow τ1 τ2 => interp_arrow (interp τ1) (interp τ2)
-    | TVar x => ctx_lookup x
-    | TRec τ' => interp_rec (interp τ')
-    | TUnknown => interp_unknown'
-    end.
   Notation "⟦ τ ⟧" := (interp τ). (** the actual relations on values *)
 
+  (* boring lemma's related to foldings {{{ *)
+
+  Lemma unfold_interp : interp ≡ interp_gen_ne interp.
+  Proof. apply fixpoint_unfold. Qed.
+
+  Lemma unfold_interp_type τ : interp τ ≡ interp_gen_ne interp τ.
+  Proof. f_equiv. apply unfold_interp. Qed.
+
+  Lemma unfold_interp_type_pair τ vv : interp τ vv ≡ interp_gen interp τ vv.
+  Proof. assert (H : interp_gen interp τ vv ≡ interp_gen_ne interp τ vv). auto_equiv. rewrite H. apply unfold_interp_type. Qed.
+
+  Lemma interp_rw_TUnit ww : interp TUnit ww ≡
+    (⌜ww.1 = stlc_mu.lang.UnitV⌝ ∧ ⌜ww.2 = cast_calculus.lang.UnitV⌝)%I.
+  Proof. by rewrite (unfold_interp_type_pair TUnit). Qed.
+
+  Lemma interp_rw_TProd τ1 τ2 ww : interp (TProd τ1 τ2) ww ≡
+    (∃ v1v1' v2v2', ⌜ww = (stlc_mu.lang.PairV (v1v1'.1) (v2v2'.1), cast_calculus.lang.PairV (v1v1'.2) (v2v2'.2))⌝ ∧
+                                  interp τ1 v1v1' ∧ interp τ2 v2v2')%I.
+  Proof. rewrite (unfold_interp_type_pair (TProd τ1 τ2)). simpl. auto_equiv; by rewrite -unfold_interp_type_pair. Qed.
+
+  Lemma interp_rw_TSum τ1 τ2 ww : interp (TSum τ1 τ2) ww ≡
+    ((∃ vv', ⌜ww = (stlc_mu.lang.InjLV (vv'.1), InjLV (vv'.2))⌝ ∧ interp τ1 vv') ∨
+                    (∃ vv', ⌜ww = (stlc_mu.lang.InjRV (vv'.1), InjRV (vv'.2))⌝ ∧ interp τ2 vv'))%I.
+  Proof. rewrite (unfold_interp_type_pair (TSum τ1 τ2)). simpl. auto_equiv; by rewrite -unfold_interp_type_pair. Qed.
+
+  Lemma interp_gen_interp_gen_ne Ψ τ ww : interp_gen Ψ τ ww ≡ interp_gen_ne Ψ τ ww.
+  Proof. auto. Qed.
+
+  Lemma interp_rw_TArrow τ1 τ2 ww : interp (TArrow τ1 τ2) ww ≡
+    (□ ∀ vv, interp τ1 vv →
+             interp_expr
+               (interp τ2) (stlc_mu.lang.App (stlc_mu.lang.of_val (ww.1)) (stlc_mu.lang.of_val (vv.1)),
+                        cast_calculus.lang.App (cast_calculus.lang.of_val (ww.2)) (cast_calculus.lang.of_val (vv.2))))%I.
+  Proof. rewrite (unfold_interp_type_pair (TArrow τ1 τ2)). simpl.
+         f_equiv. f_equiv.  intro. f_equiv. by rewrite -unfold_interp_type_pair.
+         rewrite /interp_expr. auto_equiv. by rewrite unfold_interp_type_pair.
+  Qed.
+
+  Lemma interp_rw_TRec τb ww : interp (TRec τb) ww ≡
+    (□ ∃ w w', ⌜ww = (stlc_mu.lang.FoldV w, cast_calculus.lang.FoldV w')⌝ ∧ ▷ interp (τb.[TRec τb/]) (w, w'))%I.
+  Proof. rewrite (unfold_interp_type_pair). by simpl. Qed.
+
+  Lemma interp_rw_TUnknown ww : interp TUnknown ww ≡
+    (∃ v v', □ (
+                               (⌜ ww = (embedV_TUnit v , castupV_TUnit v') ⌝                   ∧ ▷ interp TUnit (v, v') )
+                             ∨ (⌜ ww = (embedV_Ground_TProd v , castupV_TProd v') ⌝            ∧ ▷ interp (TProd TUnknown TUnknown) (v , v'))
+                             ∨ (⌜ ww = (embedV_Ground_TSum v , castupV_TSum v') ⌝              ∧ ▷ interp (TSum TUnknown TUnknown) (v , v'))
+                             ∨ (⌜ ww = (embedV_Ground_TArrow v , castupV_TArrow v') ⌝          ∧ ▷ interp (TArrow TUnknown TUnknown) (v , v'))
+                             ∨ (∃ u u', ⌜ ww = (embedV_TUnknown u, castupV_TRec (FoldV u')) ⌝ ∧ ▷ interp TUnknown (u , u')
+                               )))%I.
+  Proof. rewrite (unfold_interp_type_pair). by simpl. Qed.
+
+  (* }}} *)
+
+  Global Instance interp_persistent τ vv :
+    Persistent (⟦ τ ⟧ vv).
+  Proof.
+    revert vv. induction τ; intro p; rewrite unfold_interp_type_pair; simpl; try by apply _.
+    - apply exist_persistent. intro q. apply exist_persistent. intro r.
+      do 2 rewrite -unfold_interp_type_pair. apply _.
+    - apply or_persistent; apply exist_persistent; intro q; rewrite -unfold_interp_type_pair; apply _.
+  Qed.
+
+
   Definition interp_env (Γ : list type)
-      (Δ : listO D) (vvs : list (stlc_mu.lang.val * cast_calculus.lang.val)) : iProp Σ :=
-    (⌜length Γ = length vvs⌝ ∗ [∗] zip_with (λ τ, ⟦ τ ⟧ Δ) Γ vvs)%I.
+      (vvs : list (stlc_mu.lang.val * cast_calculus.lang.val)) : iProp Σ :=
+    (⌜length Γ = length vvs⌝ ∗ [∗] zip_with (λ τ, ⟦ τ ⟧) Γ vvs)%I.
   Notation "⟦ Γ ⟧*" := (interp_env Γ).
 
-  Class env_Persistent Δ :=
-    ctx_persistentP : Forall (λ τi, ∀ vv, Persistent (τi vv)) Δ.
-  Global Instance ctx_persistent_nil : env_Persistent [].
-  Proof. by constructor. Qed.
-  Global Instance ctx_persistent_cons τi Δ :
-    (∀ vv, Persistent (τi vv)) → env_Persistent Δ → env_Persistent (τi :: Δ).
-  Proof. by constructor. Qed.
-  Global Instance ctx_persistent_lookup Δ x vv :
-    env_Persistent Δ → Persistent (ctx_lookup x Δ vv).
-  Proof. intros HΔ; revert x; induction HΔ=>-[|?] /=; apply _. Qed.
-  Global Instance interp_persistent τ Δ vv :
-    env_Persistent Δ → Persistent (⟦ τ ⟧ Δ vv).
+  Global Instance interp_env_base_persistent Γ vs :
+  TCForall Persistent (zip_with (λ τ, ⟦ τ ⟧) Γ vs).
   Proof.
-    revert vv Δ; induction τ=> vv Δ HΔ; simpl; try apply _.
-    - rewrite /Persistent fixpoint_interp_rec1_eq.
-      rewrite /interp_rec1.
-      rewrite /= intuitionistically_into_persistently.
-      by apply persistently_intro'.
-    - rewrite /Persistent /interp_unknown_pre'.
-      rewrite unfold_fixpoint_interp_unknown1'.
-      rewrite /= intuitionistically_into_persistently.
-      apply persistently_intro'.
-      done. done.
-  Qed.
-
-  Global Instance interp_env_base_persistent Δ Γ vs :
-  env_Persistent Δ → TCForall Persistent (zip_with (λ τ, ⟦ τ ⟧ Δ) Γ vs).
-  Proof.
-    intros HΔ. revert vs.
+    revert vs.
     induction Γ => vs; simpl; destruct vs; constructor; apply _.
   Qed.
-  Global Instance interp_env_persistent Γ Δ vvs :
-    env_Persistent Δ → Persistent (⟦ Γ ⟧* Δ vvs) := _.
+  Global Instance interp_env_persistent Γ vvs :
+    Persistent (⟦ Γ ⟧* vvs) := _.
 
-  Lemma interp_weaken Δ1 Π Δ2 τ :
-    ⟦ τ.[upn (length Δ1) (ren (+ length Π))] ⟧ (Δ1 ++ Π ++ Δ2)
-    ≡ ⟦ τ ⟧ (Δ1 ++ Δ2).
-  Proof.
-    revert Δ1 Π Δ2. induction τ=> Δ1 Π Δ2; simpl; auto.
-    - intros ww; simpl; properness; auto. by apply IHτ1. by apply IHτ2.
-    - intros ww; simpl; properness; auto. by apply IHτ1. by apply IHτ2.
-    - unfold interp_expr.
-      intros ww; simpl; properness; auto. by apply IHτ1. by apply IHτ2.
-    - apply fixpoint_proper=> τi ww /=.
-      properness; auto. apply (IHτ (_ :: _)).
-    - rewrite iter_up; destruct lt_dec as [Hl | Hl]; simpl.
-      { by rewrite !lookup_app_l. }
-      (* FIXME: Ideally we wouldn't have to do this kinf of surgery. *)
-      change (bi_ofeO (uPredI (iResUR Σ))) with (uPredO (iResUR Σ)).
-      rewrite !lookup_app_r; [|lia ..]. do 2 f_equiv. lia.
-  Qed.
-
-  Lemma interp_subst_up Δ1 Δ2 τ τ' :
-    ⟦ τ ⟧ (Δ1 ++ interp τ' Δ2 :: Δ2)
-    ≡ ⟦ τ.[upn (length Δ1) (τ' .: ids)] ⟧ (Δ1 ++ Δ2).
-  Proof.
-    revert Δ1 Δ2; induction τ=> Δ1 Δ2; simpl; auto.
-    - intros ww; simpl; properness; auto. by apply IHτ1. by apply IHτ2.
-    - intros ww; simpl; properness; auto. by apply IHτ1. by apply IHτ2.
-    - unfold interp_expr.
-      intros ww; simpl; properness; auto. by apply IHτ1. by apply IHτ2.
-    - apply fixpoint_proper=> τi ww /=.
-      properness; auto. apply (IHτ (_ :: _)).
-    - rewrite iter_up; destruct lt_dec as [Hl | Hl]; simpl.
-      { by rewrite !lookup_app_l. }
-      (* FIXME: Ideally we wouldn't have to do this kinf of surgery. *)
-      change (bi_ofeO (uPredI (iResUR Σ))) with (uPredO (iResUR Σ)).
-      rewrite !lookup_app_r; [|lia ..].
-      case EQ: (x - length Δ1) => [|n]; simpl.
-      { symmetry. asimpl. apply (interp_weaken [] Δ1 Δ2 τ'). }
-      change (bi_ofeO (uPredI (iResUR Σ))) with (uPredO (iResUR Σ)).
-      rewrite !lookup_app_r; [|lia ..]. do 2 f_equiv. lia.
-  Qed.
-
-  Lemma interp_subst Δ2 τ τ' v : ⟦ τ ⟧ (⟦ τ' ⟧ Δ2 :: Δ2) v ≡ ⟦ τ.[τ'/] ⟧ Δ2 v.
-  Proof. apply (interp_subst_up []). Qed.
-
-  Lemma interp_env_length Δ Γ vvs : bi_entails (⟦ Γ ⟧* Δ vvs) (⌜length Γ = length vvs⌝).
+  Lemma interp_env_length Γ vvs : ⟦ Γ ⟧* vvs ⊢ ⌜length Γ = length vvs⌝.
   Proof. by iIntros "[% ?]". Qed.
 
-  Lemma interp_env_Some_l Δ Γ vvs x τ :
-    Γ !! x = Some τ → bi_entails (⟦ Γ ⟧* Δ vvs) (∃ vv, ⌜vvs !! x = Some vv⌝ ∧ ⟦ τ ⟧ Δ vv).
+  Lemma interp_env_Some_l Γ vvs x τ :
+    Γ !! x = Some τ → ⟦ Γ ⟧* vvs ⊢ (∃ vv, ⌜vvs !! x = Some vv⌝ ∧ ⟦ τ ⟧ vv).
   Proof.
     iIntros (?) "[Hlen HΓ]"; iDestruct "Hlen" as %Hlen.
     destruct (lookup_lt_is_Some_2 vvs x) as [v Hv].
@@ -374,21 +202,13 @@ Section logrel.
     rewrite lookup_zip_with; by simplify_option_eq.
   Qed.
 
-  Lemma interp_env_nil Δ : ⊢ ⟦ [] ⟧* Δ [].
+  Lemma interp_env_nil : ⊢ ⟦ [] ⟧* [].
   Proof. iSplit; simpl; auto. Qed.
-  Lemma interp_env_cons Δ Γ vvs τ vv :
-    ⟦ τ :: Γ ⟧* Δ (vv :: vvs) ⊣⊢ ⟦ τ ⟧ Δ vv ∗ ⟦ Γ ⟧* Δ vvs.
+  Lemma interp_env_cons Γ vvs τ vv :
+    ⟦ τ :: Γ ⟧* (vv :: vvs) ⊣⊢ ⟦ τ ⟧ vv ∗ ⟦ Γ ⟧* vvs.
   Proof.
-    rewrite /interp_env /= (assoc _ (⟦ _ ⟧ _ _)) -(comm _ ⌜_ = _⌝%I) -assoc.
+    rewrite /interp_env /= (assoc _ (⟦ _ ⟧ _)) -(comm _ ⌜_ = _⌝%I) -assoc.
     by apply sep_proper; [apply pure_proper; lia|].
-  Qed.
-
-  Lemma interp_env_ren Δ (Γ : list type) vvs τi :
-    ⟦ subst (ren (+1)) <$> Γ ⟧* (τi :: Δ) vvs ⊣⊢ ⟦ Γ ⟧* Δ vvs.
-  Proof.
-    apply sep_proper; [apply pure_proper; by rewrite fmap_length|].
-    revert Δ vvs τi; induction Γ=> Δ [|v vs] τi; csimpl; auto.
-    apply sep_proper; auto. apply (interp_weaken [] [τi] Δ).
   Qed.
 
 End logrel.
@@ -406,8 +226,7 @@ Section bin_log_def.
 
   Definition bin_log_related
   (Γ : list cast_calculus.types.type) (e : stlc_mu.lang.expr) (e' : cast_calculus.lang.expr) (τ : cast_calculus.types.type) :=
-    ∀ Δ vvs (ei' : cast_calculus.lang.expr), env_Persistent Δ →
-    initially_inv ei' ∗ ⟦ Γ ⟧* Δ vvs ⊢
-    ⟦ τ ⟧ₑ Δ (e.[stlc_mu.typing.env_subst (vvs.*1)], e'.[cast_calculus.typing.env_subst (vvs.*2)]).
+    ∀ vvs (ei' : cast_calculus.lang.expr),
+    initially_inv ei' ∗ ⟦ Γ ⟧* vvs ⊢
+    ⟦ τ ⟧ₑ (e.[stlc_mu.typing.env_subst (vvs.*1)], e'.[cast_calculus.typing.env_subst (vvs.*2)]).
 End bin_log_def.
-
