theories/backtranslation/expressions.v
@@ -1,6 +1,7 @@
-From fae_gtlc_mu.cast_calculus Require Import lang.
+From fae_gtlc_mu.cast_calculus Require Import lang consistency.standard consistency.equivalence.proof.
 From fae_gtlc_mu.stlc_mu Require Import lang.
 From fae_gtlc_mu.backtranslation Require Import cast_help.general.
+From fae_gtlc_mu.cast_calculus Require Import types.
 
 Reserved Notation "<< e >>" (at level 4, e at next level).
 Fixpoint backtranslate_expr (e : cast_calculus.lang.expr) : expr :=
@@ -18,8 +19,8 @@ Fixpoint backtranslate_expr (e : cast_calculus.lang.expr) : expr :=
   | cast_calculus.lang.Fold e => Fold <<e>>
   | cast_calculus.lang.Unfold e => Unfold <<e>>
   | Cast e τi τf =>
-    match (cons_stand_dec τi τf, decide (TClosed τi) , decide (TClosed τf)) with
-    | (inl pC , left pi, left pf) => 𝓕c (cons_co τi pi τf pf pC) [] <<e>>
+    match (decide (cons_stand_open τi τf), decide (TClosed τi) , decide (TClosed τf)) with
+    | (left pC , left pi, left pf) => (𝓕 (cons_co τi pi τf pf pC)) <<e>>
     | _ => Unit
     end
   | Blame => Ω
