theories/cast_calculus/consistency/equivalence/proof.v
@@ -1,0 +1,5 @@
+From fae_gtlc_mu Require Import prelude.
+From fae_gtlc_mu.cast_calculus.consistency Require Import standard structural.
+
+Lemma cons_co τi pτi τf pτf : cons_stand τi pτi τf pτf → cons_struct [] τi τf.
+Admitted.
