theories/refinements/static_gradual/compat_cast/arrow_arrow.v
@@ -1,10 +1,10 @@
-From fae_gtlc_mu.refinements.static_gradual Require Export tactics_left logical_relation resources_right compat_easy help_left compat_cast.defs.
+From fae_gtlc_mu.refinements.static_gradual Require Export logical_relation resources_right compat_easy help_left compat_cast.defs.
 From fae_gtlc_mu.cast_calculus Require Export types typing.
 From fae_gtlc_mu.stlc_mu Require Export lang.
 From iris.algebra Require Import list.
 From iris.proofmode Require Import tactics.
 From iris.program_logic Require Import lifting.
-From fae_gtlc_mu.cast_calculus Require Export consistency.structural.definition.
+From fae_gtlc_mu.cast_calculus Require Export consistency.structural.
 From fae_gtlc_mu.backtranslation Require Export cast_help.general cast_help.extract cast_help.embed.
 From fae_gtlc_mu.cast_calculus Require Export lang types.
 
@@ -29,16 +29,17 @@ Section compat_cast_arrow_arrow.
   (* Qed. *)
 
   Lemma back_cast_ar_arrow_arrow:
-    ∀ (A : list (type * type)) (τ1 τ2 τ3 τ4 : type) (pC1 : A ⊢ τ3 ~ τ1) (pC2 : A ⊢ τ2 ~ τ4)
+    ∀ (A : list (type * type)) (τ1 τ1' τ2 τ2' : type) (pC1 : cons_struct A τ1' τ1) (pC2 : cons_struct A τ2 τ2')
       (IHpC1 : back_cast_ar pC1) (IHpC2 : back_cast_ar pC2),
-      back_cast_ar (consTArrowTArrow A τ1 τ2 τ3 τ4 pC1 pC2).
+      back_cast_ar (consTArrowTArrow A τ1 τ1' τ2 τ2' pC1 pC2).
   Proof.
-    intros A τ1 τ2 τ3 τ4 pC1 pC2 IHpC1 IHpC2.
+    intros A τ1 τ1' τ2 τ2' pC1 pC2 IHpC1 IHpC2.
     rewrite /back_cast_ar. iIntros (ei' K' v v' fs) "(#Hfs & #Hvv' & #Hei' & Hv')".
     fold interp.
     iDestruct "Hfs" as "[% Hfs']"; iAssert (rel_cast_functions A fs) with "[Hfs']" as "Hfs". iSplit; done. iClear "Hfs'".
     rewrite /𝓕c /𝓕. fold (𝓕 pC1) (𝓕 pC2). rewrite between_TArrow_subst_rewrite.
-    rename v into f. rename v' into f'. iDestruct "Hv'" as "Hf'". iDestruct "Hvv'" as "Hff'". iClear "Hvv'".
+    rename v into f. rename v' into f'. iDestruct "Hv'" as "Hf'". iDestruct "Hvv'" as "Hff'".
+    (* iClear "Hvv'". *)
     fold (𝓕c pC1 fs) (𝓕c pC2 fs).
     iDestruct "Hfs" as "[% Hfs']"; iAssert (rel_cast_functions A fs) with "[Hfs']" as "Hfs". iSplit; done. iClear "Hfs'".
     do 2 rewrite 𝓕c_rewrite.
@@ -46,8 +47,10 @@ Section compat_cast_arrow_arrow.
     wp_head.
     asimpl.
     iApply wp_value.
-    iExists (CastV f' (TArrow τ1 τ2) (TArrow τ3 τ4) (Between_arrow_types τ1 τ2 τ3 τ4)).
-    iSplitL "Hf'"; first done.
+    iExists (CastV f' (TArrow τ1 τ2) (TArrow τ1' τ2') (TArrow_TArrow_icp τ1 τ2 τ1' τ2')).
+    rewrite interp_rw_TArrow.
+    iSplitL "Hf'"; auto.
+    rewrite interp_rw_TArrow.
     iModIntro.
     (** actual thing to prove *)
     (** ===================== *)
@@ -59,14 +62,14 @@ Section compat_cast_arrow_arrow.
     wp_head. asimpl.
     (** specification *)
     iMod (step_pure _ ei' K'
-                    (App (Cast (# f') (TArrow τ1 τ2) (TArrow τ3 τ4)) (# a'))
-                    (Cast (App (# f') (Cast (# a') τ3 τ1)) τ2 τ4) with "[Hf']") as "Hf'".
+                    (App (Cast (# f') (TArrow τ1 τ2) (TArrow τ1' τ2')) (# a'))
+                    (Cast (App (# f') (Cast (# a') τ1' τ1)) τ2 τ2') with "[Hf']") as "Hf'".
     intros. eapply AppCast; try by rewrite -to_of_val. auto. by iFrame.
     (** first IH for the arguments *)
     iApply (wp_bind (fill $ [stlc_mu.lang.AppRCtx _ ; stlc_mu.lang.AppRCtx _])).
     iApply (wp_wand with "[-]").
     rewrite -𝓕c_rewrite.
-    iApply (IHpC1 ei' (AppRCtx f' :: CastCtx τ2 τ4 :: K') with "[Hf']").
+    iApply (IHpC1 ei' (AppRCtx f' :: CastCtx τ2 τ2' :: K') with "[Hf']").
     (* iApply (IHpC1 ei' (CastCtx τ2 τ4 :: AppRCtx f' :: K') with "[Hf']"). *)
     iSplitR. done.
     iSplitR. done.
@@ -80,7 +83,7 @@ Section compat_cast_arrow_arrow.
     iApply (wp_bind (fill $ [stlc_mu.lang.AppRCtx _ ])).
     iApply (wp_wand with "[-]").
     iDestruct ("Hff'" with "Hbb'") as "Hfbf'b' /=".
-    iApply ("Hfbf'b'" $! (CastCtx τ2 τ4 :: K')).
+    iApply ("Hfbf'b'" $! (CastCtx τ2 τ2' :: K')).
     simpl.
     iExact "Hb'".
     iIntros (r) "HHH". iDestruct "HHH" as (r') "[Hr' Hrr']".
@@ -95,7 +98,8 @@ Section compat_cast_arrow_arrow.
     iSplitR. done.
     done.
     iIntros (s) "HHH". done.
-  Admitted.
+    Unshelve. all:apply hack.
+  Qed.
 
 
 End compat_cast_arrow_arrow.
