theories/refinements/static_gradual/compat_cast/ground_star.v
@@ -1,13 +1,12 @@
-From fae_gtlc_mu.refinements.static_gradual Require Export logical_relation resources_right compat_easy help_left compat_cast.defs compat_cast.extract_embed.
+From fae_gtlc_mu.refinements.static_gradual Require Export logical_relation resources_right compat_easy help_left compat_cast.defs.
 From fae_gtlc_mu.stlc_mu Require Export lang.
 From fae_gtlc_mu.cast_calculus Require Export lang.
 From iris.algebra Require Import list.
 From iris.proofmode Require Import tactics.
 From iris.program_logic Require Import lifting.
 From fae_gtlc_mu.cast_calculus Require Export types.
-From fae_gtlc_mu.cast_calculus Require Export consistency.structural.definition.
+From fae_gtlc_mu.cast_calculus Require Export consistency.structural.
 From fae_gtlc_mu.backtranslation Require Export cast_help.general cast_help.extract cast_help.embed.
-From fae_gtlc_mu.refinements.static_gradual Require Export tactics_left.
 From fae_gtlc_mu.cast_calculus Require Export types typing.
 
 Section ground_star.
@@ -22,10 +21,10 @@ Section ground_star.
   Local Hint Resolve to_of_val : core.
   Local Hint Resolve stlc_mu.lang.to_of_val : core.
 
-  Lemma refold_interp_unknown' vv' : fixpoint interp_unknown1' vv' ≡ interp TUnknown [] vv'.
-  Proof.
-    auto.
-  Qed.
+  (* Lemma refold_interp_unknown' vv' : fixpoint interp_unknown1' vv' ≡ interp TUnknown [] vv'. *)
+  (* Proof. *)
+  (*   auto. *)
+  (* Qed. *)
 
 
   Lemma back_cast_ar_ground_star:
@@ -34,20 +33,20 @@ Section ground_star.
     intros A τG G.
     rewrite /back_cast_ar /𝓕c /𝓕. iIntros (ei' K' v v' fs) "(#Hfs & #Hvv' & #Hei' & Hv')". rewrite embed_no_subs.
     destruct G; rewrite /𝓕c /𝓕.
-      + iDestruct "Hvv'" as "%". simpl in H. inversion H. rewrite H0 H1. clear v v' H H0 H1.
+      + rewrite interp_rw_TUnit. iDestruct "Hvv'" as "%". simpl in H. inversion H. rewrite H0 H1. clear v v' H H0 H1.
         wp_head. asimpl. wp_value.
-        iExists (CastV UnitV _ _ (From_ground_to_unknown _ Ground_TUnit)). iSplitL. done.
-        rewrite unfold_fixpoint_interp_unknown1'. simpl. iModIntro.
-        iLeft. done. constructor.
+        iExists (CastV UnitV _ _ (TGround_TUnknown_icp Ground_TUnit)). iSplitL. done.
+        rewrite interp_rw_TUnknown. iExists _, _. simpl. iModIntro.
+        iLeft. simpl. done. constructor.
       + iDestruct "Hvv'" as ((v1 , v1') (v2 , v2')) "[% [H1 H2]]". simpl in H; inversion H; clear H H1 H2 v v'.
         wp_head. asimpl. wp_value.
-        iExists (CastV (PairV v1' v2') _ _ (From_ground_to_unknown _ Ground_TProd)). iSplitL. done.
+        iExists (CastV (PairV v1' v2') _ _ (TGround_TUnknown_icp _ Ground_TProd)). iSplitL. done.
         rewrite (unfold_fixpoint_interp_unknown1' [] (stlc_mu.lang.FoldV (stlc_mu.lang.InjLV (stlc_mu.lang.InjLV (stlc_mu.lang.InjRV (stlc_mu.lang.PairV v1 v2)))),
-    CastV (PairV v1' v2') (⋆ × ⋆) ⋆ (From_ground_to_unknown (⋆ × ⋆) Ground_TProd))).
+    CastV (PairV v1' v2') (⋆ × ⋆) ⋆ (TGround_TUnknown_icp (⋆ × ⋆) Ground_TProd))).
         iModIntro. iRight. iLeft.
         iExists v1 , v1' , v2 , v2'. iSplit. done. iSplit; done.
       + wp_head. asimpl. wp_value.
-        iExists (CastV v' _ _ (From_ground_to_unknown _ Ground_TSum)).
+        iExists (CastV v' _ _ (TGround_TUnknown_icp _ Ground_TSum)).
         iSplitL. done. rewrite unfold_fixpoint_interp_unknown1'.
         iModIntro. iRight. iRight. iLeft.
         iDestruct "Hvv'" as "[H1 | H2]".
@@ -59,7 +58,7 @@ Section ground_star.
           iRight. iExists v2 , v2'. iSplit. done. auto.
         * constructor.
       + iDestruct "Hvv'" as "#Hvv'". wp_head. asimpl. wp_value.
-        iExists (CastV v' _ _ (From_ground_to_unknown _ Ground_TArrow)). iSplitL. done.
+        iExists (CastV v' _ _ (TGround_TUnknown_icp _ Ground_TArrow)). iSplitL. done.
         rewrite unfold_fixpoint_interp_unknown1'.
         iModIntro. iRight. iRight. iRight. iLeft.
         iExists v , v'. iSplit. done. iModIntro. iModIntro.
@@ -77,11 +76,12 @@ Section ground_star.
         (** boring steps *)
         iApply (wp_bind (fill $ [stlc_mu.lang.InjRCtx ; stlc_mu.lang.FoldCtx])).
         wp_head. wp_value. simpl. wp_value.
-        iExists (CastV (FoldV u') _ _ (From_ground_to_unknown _ Ground_TRec)).
+        iExists (CastV (FoldV u') _ _ (TGround_TUnknown_icp _ Ground_TRec)).
         iSplitL. done.
-        rewrite (unfold_fixpoint_interp_unknown1' [] (stlc_mu.lang.FoldV (stlc_mu.lang.InjRV u), CastV (FoldV u') (TRec ⋆) ⋆ (From_ground_to_unknown (TRec ⋆) Ground_TRec))).
+        rewrite (unfold_fixpoint_interp_unknown1' [] (stlc_mu.lang.FoldV (stlc_mu.lang.InjRV u), CastV (FoldV u') (TRec ⋆) ⋆ (TGround_TUnknown_icp (TRec ⋆) Ground_TRec))).
         iModIntro. iRight. iRight. iRight. iRight.
         iExists u , u'. iSplit; done.
+        (* Unshelve. apply (@ectx_lang_ctx stlc_mu.lang.ectx_lang _). *)
   Admitted.
 
 
