theories/refinements/static_gradual/compat_cast/prod_prod.v
@@ -1,10 +1,10 @@
-From fae_gtlc_mu.refinements.static_gradual Require Export tactics_left logical_relation resources_right compat_easy help_left compat_cast.defs.
+From fae_gtlc_mu.refinements.static_gradual Require Export logical_relation resources_right compat_easy help_left compat_cast.defs.
 From fae_gtlc_mu.cast_calculus Require Export types typing.
 From fae_gtlc_mu.stlc_mu Require Export lang.
 From iris.algebra Require Import list.
 From iris.proofmode Require Import tactics.
 From iris.program_logic Require Import lifting.
-From fae_gtlc_mu.cast_calculus Require Export consistency.structural.definition.
+From fae_gtlc_mu.cast_calculus Require Export consistency.structural.
 From fae_gtlc_mu.backtranslation Require Export cast_help.general cast_help.extract cast_help.embed.
 From fae_gtlc_mu.cast_calculus Require Export lang types.
 
@@ -29,7 +29,7 @@ Section compat_cast_prod_prod.
   (* Qed. *)
 
   Lemma back_cast_ar_prod_prod:
-    ∀ (A : list (type * type)) (τ1 τ1' τ2 τ2' : type) (pC1 : A ⊢ τ1 ~ τ1') (pC2 : A ⊢ τ2 ~ τ2')
+    ∀ (A : list (type * type)) (τ1 τ1' τ2 τ2' : type) (pC1 : cons_struct A τ1 τ1') (pC2 : cons_struct A τ2 τ2')
       (IHpC1 : back_cast_ar pC1) (IHpC2 : back_cast_ar pC2),
       back_cast_ar (consTProdTProd A τ1 τ1' τ2 τ2' pC1 pC2).
   Proof.
@@ -37,10 +37,12 @@ Section compat_cast_prod_prod.
     rewrite /back_cast_ar. iIntros (ei' K' v v' fs) "(#Hfs & #Hvv' & #Hei' & Hv')".
     iDestruct "Hfs" as "[% Hfs']"; iAssert (rel_cast_functions A fs) with "[Hfs']" as "Hfs". iSplit; done. iClear "Hfs'".
     rewrite /𝓕c /𝓕. fold (𝓕 pC1) (𝓕 pC2). rewrite between_TProd_subst_rewrite.
+    rewrite interp_rw_TProd.
     iDestruct "Hvv'" as ((v1, v1') (v2, v2')) "(% & #H1 & #H2)". simpl in H0. inversion H0. clear H0 H2 H3 v v'.
     iDestruct "Hfs" as "[% Hfs']"; iAssert (rel_cast_functions A fs) with "[Hfs']" as "Hfs". iSplit; done. iClear "Hfs'".
     fold interp.
     fold (𝓕c pC1 fs) (𝓕c pC2 fs).
+
     wp_head. asimpl.
     rewrite 𝓕c_rewrite.
     (** boring steps implementation side *)
@@ -85,8 +87,9 @@ Section compat_cast_prod_prod.
     iIntros (v2f) "HHH". iDestruct "HHH" as (v2f') "[Hvf #Hv2fv2f']". simpl.
     wp_value.
     iExists (PairV v1f' v2f'). iSplitL. done.
+    rewrite interp_rw_TProd.
     iExists (v1f , v1f') , (v2f , v2f') . iSplitR. done. by iSplit.
-  Admitted.
-
+    Unshelve. all:apply hack.
+Qed.
 
 End compat_cast_prod_prod.
