theories/refinements/static_gradual/compat_cast/sum_sum.v
@@ -1,10 +1,10 @@
-From fae_gtlc_mu.refinements.static_gradual Require Export tactics_left logical_relation resources_right compat_easy help_left compat_cast.defs.
+From fae_gtlc_mu.refinements.static_gradual Require Export logical_relation resources_right compat_easy help_left compat_cast.defs.
 From fae_gtlc_mu.cast_calculus Require Export types typing.
 From fae_gtlc_mu.stlc_mu Require Export lang.
 From iris.algebra Require Import list.
 From iris.proofmode Require Import tactics.
 From iris.program_logic Require Import lifting.
-From fae_gtlc_mu.cast_calculus Require Export consistency.structural.definition.
+From fae_gtlc_mu.cast_calculus Require Export consistency.structural.
 From fae_gtlc_mu.backtranslation Require Export cast_help.general cast_help.extract cast_help.embed.
 From fae_gtlc_mu.cast_calculus Require Export lang types.
 
@@ -29,7 +29,7 @@ Section compat_cast_sum_sum.
   (* Qed. *)
 
   Lemma back_cast_ar_sum_sum:
-    ∀ (A : list (type * type)) (τ1 τ1' τ2 τ2' : type) (pC1 : A ⊢ τ1 ~ τ1') (pC2 : A ⊢ τ2 ~ τ2')
+    ∀ (A : list (type * type)) (τ1 τ1' τ2 τ2' : type) (pC1 : cons_struct A τ1 τ1') (pC2 : cons_struct A τ2 τ2')
       (IHpC1 : back_cast_ar pC1) (IHpC2 : back_cast_ar pC2),
       back_cast_ar (consTSumTSum A τ1 τ1' τ2 τ2' pC1 pC2).
   Proof.
@@ -37,11 +37,13 @@ Section compat_cast_sum_sum.
     rewrite /back_cast_ar. iIntros (ei' K' v v' fs) "(#Hfs & #Hvv' & #Hei' & Hv')".
     iDestruct "Hfs" as "[% Hfs']"; iAssert (rel_cast_functions A fs) with "[Hfs']" as "Hfs". iSplit; done. iClear "Hfs'".
     rewrite /𝓕c /𝓕. fold (𝓕 pC1) (𝓕 pC2). rewrite between_TSum_subst_rewrite.
-    wp_head. asimpl.
+    wp_head.
+    asimpl.
     iMod (step_pure _ ei' K'
                     (Cast (# v') (τ1 + τ2)%type (τ1' + τ2')%type)
                     (Case (# v') (InjL (Cast (Var 0) τ1 τ1')) (InjR (Cast (Var 0) τ2 τ2'))) with "[Hv']") as "Hv'".
     intros. eapply SumCast. by simplify_option_eq. auto. iSplitR; try done.
+    rewrite interp_rw_TSum.
     iDestruct "Hvv'" as "[H1 | H2]".
     + iDestruct "H1" as ((v1 , v1')) "[% Hv1v1']". inversion H0. clear H0 H2 H3 v v'.
       wp_head. asimpl.
@@ -53,9 +55,10 @@ Section compat_cast_sum_sum.
       iSplitR; try done.
       iSplitR; try done.
       iIntros (v1f) "HHH". iDestruct "HHH" as (v1f') "[Hv1f' Hv1fv1f']".
-      wp_value.
+      iApply wp_value.
       iExists (InjLV v1f').
       iSplitL "Hv1f'". done.
+      rewrite interp_rw_TSum.
       iLeft. iExists (v1f , v1f'). by iFrame.
     + iDestruct "H2" as ((v1 , v1')) "[% Hv1v1']". inversion H0. clear H0 H2 H3 v v'.
       wp_head. asimpl.
@@ -67,11 +70,13 @@ Section compat_cast_sum_sum.
       iSplitR; try done.
       iSplitR; try done.
       iIntros (v1f) "HHH". iDestruct "HHH" as (v1f') "[Hv1f' Hv1fv1f']".
-      wp_value.
+      iApply wp_value.
       iExists (InjRV v1f').
       iSplitL "Hv1f'". done.
+      rewrite interp_rw_TSum.
       iRight. iExists (v1f , v1f'). by iFrame.
-  Admitted.
+      Unshelve. all: apply hack.
+  Qed.
 
 
 End compat_cast_sum_sum.
