theories/refinements/static_gradual/compat_easy.v
@@ -24,13 +24,12 @@ Section fundamental.
     iIntros (v); iDestruct 1 as (w) Hv.
 
   (* Put all quantifiers at the outer level *)
-  Lemma bin_log_related_alt {Γ e e' τ} : Γ ⊨ e ≤log≤ e' : τ → ∀ Δ vvs ei' K',
-    env_Persistent Δ →
-    initially_inv ei' ∗ ⟦ Γ ⟧* Δ vvs ∗ currently_half (fill K' (e'.[cast_calculus.typing.env_subst (vvs.*2)]))
+  Lemma bin_log_related_alt {Γ e e' τ} : Γ ⊨ e ≤log≤ e' : τ → ∀ vvs ei' K',
+    initially_inv ei' ∗ ⟦ Γ ⟧* vvs ∗ currently_half (fill K' (e'.[cast_calculus.typing.env_subst (vvs.*2)]))
     ⊢ WP e.[stlc_mu.typing.env_subst (vvs.*1)] {{ v, ∃ v',
-        currently_half (fill K' (cast_calculus.lang.of_val v')) ∗ interp τ Δ (v, v') }}.
+        currently_half (fill K' (cast_calculus.lang.of_val v')) ∗ interp τ (v, v') }}.
   Proof.
-    iIntros (Hlog Δ vvs K ρ ?) "[#Hρ [HΓ Hj]]". asimpl.
+    iIntros (Hlog vvs K ρ) "[#Hρ [HΓ Hj]]". asimpl.
     iApply (Hlog with "[HΓ]"); iFrame. eauto.
   Qed.
 
@@ -39,7 +38,7 @@ Section fundamental.
   Lemma bin_log_related_var Γ x τ :
     Γ !! x = Some τ → Γ ⊨ stlc_mu.lang.Var x ≤log≤ cast_calculus.lang.Var x : τ.
   Proof.
-    iIntros (? Δ vvs ρ ?) "[#Hρ #HΓ]". iIntros (K) "Hj /=".
+    iIntros (? vvs ei') "[#Hρ #HΓ]". iIntros (K). iIntros "Hj /=".
     iDestruct (interp_env_Some_l with "HΓ") as ([v v']) "[Heq Hv]"; first done.
     iDestruct "Heq" as %Heq.
     erewrite !stlc_mu.typing.env_subst_lookup; rewrite ?list_lookup_fmap ?Heq; eauto.
@@ -49,8 +48,8 @@ Section fundamental.
 
   Lemma bin_log_related_unit Γ : Γ ⊨ stlc_mu.lang.Unit ≤log≤ cast_calculus.lang.Unit : TUnit.
   Proof.
-    iIntros (Δ vvs ρ ?) "#[Hρ HΓ]". iIntros (K) "Hj /=".
-    iApply wp_value. iExists UnitV; eauto.
+    iIntros (vvs ei') "#[Hρ HΓ]". iIntros (K) "Hj /=".
+    iApply wp_value. iExists UnitV. rewrite unfold_interp_type_pair. eauto.
   Qed.
 
   Lemma bin_log_related_pair Γ e1 e2 e1' e2' τ1 τ2
@@ -58,22 +57,24 @@ Section fundamental.
       (IHHtyped2 : Γ ⊨ e2 ≤log≤ e2' : τ2) :
     Γ ⊨ stlc_mu.lang.Pair e1 e2 ≤log≤ Pair e1' e2' : TProd τ1 τ2.
   Proof.
-    iIntros (Δ vvs ρ ?) "#[Hρ HΓ]"; iIntros (K) "Hj /=".
+    iIntros (vvs ei') "#[Hρ HΓ]"; iIntros (K) "Hj /=".
     smart_wp_bind (stlc_mu.lang.PairLCtx e2.[stlc_mu.typing.env_subst _]) v v' "[Hv #Hiv]"
-      ('`IHHtyped1 _ _ _ ((PairLCtx e2'.[env_subst _]) :: K)).
+      ('`IHHtyped1 _ _ ((PairLCtx e2'.[env_subst _]) :: K)).
     smart_wp_bind (stlc_mu.lang.PairRCtx v) w w' "[Hw #Hiw]"
-      ('`IHHtyped2 _ _ _ ((PairRCtx v') :: K)).
+      ('`IHHtyped2 _ _ ((PairRCtx v') :: K)).
     iApply wp_value.
     iExists (PairV v' w'); iFrame "Hw".
-    iExists (v, v'), (w, w'); simpl; repeat iSplit; trivial.
+    rewrite interp_rw_TProd.
+    iExists (v, v'), (w, w'). simpl; repeat iSplit; trivial.
   Qed.
 
   Lemma bin_log_related_fst Γ e e' τ1 τ2
       (IHHtyped : Γ ⊨ e ≤log≤ e' : TProd τ1 τ2) :
     Γ ⊨ stlc_mu.lang.Fst e ≤log≤ Fst e' : τ1.
   Proof.
-    iIntros (Δ vvs ρ ?) "[#Hρ #HΓ]"; iIntros (K) "Hj /=".
-    smart_wp_bind (stlc_mu.lang.FstCtx) v v' "[Hv #Hiv]" ('`IHHtyped _ _ _ (FstCtx :: K)); cbn.
+    iIntros (vvs ei') "[#Hρ #HΓ]"; iIntros (K) "Hj /=".
+    smart_wp_bind (stlc_mu.lang.FstCtx) v v' "[Hv #Hiv]" ('`IHHtyped _ _ (FstCtx :: K)); cbn.
+    rewrite interp_rw_TProd.
     iDestruct "Hiv" as ([w1 w1'] [w2 w2']) "#[% [Hw1 Hw2]]"; simplify_eq.
     iMod (step_fst _ _ K (of_val w1') (of_val w2') with "[-]") as "Hw"; eauto.
     iApply wp_pure_step_later; auto. iApply wp_value; auto.
@@ -83,8 +84,9 @@ Section fundamental.
       (IHHtyped : Γ ⊨ e ≤log≤ e' : TProd τ1 τ2) :
     Γ ⊨ stlc_mu.lang.Snd e ≤log≤ Snd e' : τ2.
   Proof.
-    iIntros (Δ vvs ρ ?) "#[Hρ HΓ]"; iIntros (K) "Hj /=".
-    smart_wp_bind (stlc_mu.lang.SndCtx) v v' "[Hv #Hiv]" ('`IHHtyped _ _ _ (SndCtx :: K)); cbn.
+    iIntros (vvs ei') "#[Hρ HΓ]"; iIntros (K) "Hj /=".
+    smart_wp_bind (stlc_mu.lang.SndCtx) v v' "[Hv #Hiv]" ('`IHHtyped _ _ (SndCtx :: K)); cbn.
+    rewrite interp_rw_TProd.
     iDestruct "Hiv" as ([w1 w1'] [w2 w2']) "#[% [Hw1 Hw2]]"; simplify_eq.
     iMod (step_snd _ _ K (of_val w1') (of_val w2') with "[-]") as "Hw"; eauto.
     iApply wp_pure_step_later; auto. iApply wp_value; auto.
@@ -94,11 +96,12 @@ Section fundamental.
       (IHHtyped : Γ ⊨ e ≤log≤ e' : τ1) :
     Γ ⊨ stlc_mu.lang.InjL e ≤log≤ InjL e' : (TSum τ1 τ2).
   Proof.
-    iIntros (Δ vvs ρ ?) "#[Hρ HΓ]"; iIntros (K) "Hj /=".
+    iIntros (vvs ei') "#[Hρ HΓ]"; iIntros (K) "Hj /=".
     smart_wp_bind (stlc_mu.lang.InjLCtx) v v' "[Hv #Hiv]"
-      ('`IHHtyped _ _ _ (InjLCtx :: K)); cbn.
+      ('`IHHtyped _ _ (InjLCtx :: K)); cbn.
     iApply wp_value. repeat rewrite /= to_of_val. eauto.
     iExists (InjLV v'); iFrame "Hv".
+    rewrite interp_rw_TSum.
     iLeft; iExists (_,_); eauto 10.
   Qed.
 
@@ -106,11 +109,12 @@ Section fundamental.
       (IHHtyped : Γ ⊨ e ≤log≤ e' : τ2) :
     Γ ⊨ stlc_mu.lang.InjR e ≤log≤ InjR e' : TSum τ1 τ2.
   Proof.
-    iIntros (Δ vvs ρ ?) "#[Hρ HΓ]"; iIntros (K) "Hj /=".
+    iIntros (vvs ei') "#[Hρ HΓ]"; iIntros (K) "Hj /=".
     smart_wp_bind (stlc_mu.lang.InjRCtx) v v' "[Hv #Hiv]"
-      ('`IHHtyped _ _ _ (InjRCtx :: K)); cbn.
+      ('`IHHtyped _ _ (InjRCtx :: K)); cbn.
     iApply wp_value. repeat rewrite /= to_of_val. eauto.
     iExists (InjRV v'); iFrame "Hv".
+    rewrite interp_rw_TSum.
     iRight; iExists (_,_); eauto 10.
   Qed.
 
@@ -124,22 +128,23 @@ Section fundamental.
       (IHHtyped3 : τ2 :: Γ ⊨ e2 ≤log≤ e2' : τ3) :
     Γ ⊨ stlc_mu.lang.Case e0 e1 e2 ≤log≤ Case e0' e1' e2' : τ3.
   Proof.
-    iIntros (Δ vvs ρ ?) "#[Hρ HΓ]"; iIntros (K) "Hj /=".
+    iIntros (vvs ei') "#[Hρ HΓ]"; iIntros (K) "Hj /=".
     iDestruct (interp_env_length with "HΓ") as %?.
     smart_wp_bind (stlc_mu.lang.CaseCtx _ _) v v' "[Hv #Hiv]"
-      ('`IHHtyped1 _ _ _ ((CaseCtx _ _) :: K)); cbn.
+      ('`IHHtyped1 _ _ ((CaseCtx _ _) :: K)); cbn.
+    rewrite interp_rw_TSum.
     iDestruct "Hiv" as "[Hiv|Hiv]".
     - iDestruct "Hiv" as ([w w']) "[% Hw]"; simplify_eq.
       iMod (step_case_inl _ _ K (of_val w') with "[-]") as "Hz"; eauto.
       simpl.
       iApply wp_pure_step_later; auto 1 using to_of_val. iNext.
-      asimpl. iApply ('`IHHtyped2 _ ((w,w') :: vvs)); repeat iSplit; eauto.
+      asimpl. iApply ('`IHHtyped2 ((w,w') :: vvs)); repeat iSplit; eauto.
       iApply interp_env_cons; auto.
     - iDestruct "Hiv" as ([w w']) "[% Hw]"; simplify_eq.
       iMod (step_case_inr _ _ K (of_val w') with "[-]") as "Hz"; eauto.
       simpl.
       iApply wp_pure_step_later; auto 1 using to_of_val. iNext.
-      asimpl. iApply ('`IHHtyped3 _ ((w,w') :: vvs)); repeat iSplit; eauto.
+      asimpl. iApply ('`IHHtyped3 ((w,w') :: vvs)); repeat iSplit; eauto.
       iApply interp_env_cons; auto.
   Qed.
 
@@ -149,13 +154,15 @@ Section fundamental.
       (IHHtyped : τ1 :: Γ ⊨ e ≤log≤ e' : τ2) :
     Γ ⊨ stlc_mu.lang.Lam e ≤log≤ Lam e' : TArrow τ1 τ2.
   Proof.
-    iIntros (Δ vvs ρ ?) "#[Hρ HΓ]"; iIntros (K) "Hj /=".
-    iApply wp_value. iExists (LamV _). iIntros "{$Hj} !#".
+    iIntros (vvs ei') "#[Hρ HΓ]"; iIntros (K) "Hj /=".
+    iApply wp_value. iExists (LamV _).
+    rewrite interp_rw_TArrow.
+    iIntros "{$Hj} !#".
     iIntros ([v v']) "#Hiv". iIntros (K') "Hj".
     iDestruct (interp_env_length with "HΓ") as %?.
     iApply wp_pure_step_later; auto 1 using to_of_val. iNext.
     iMod (step_lam _ _ K' _ (of_val v') with "[-]") as "Hz"; eauto.
-    asimpl. iApply ('`IHHtyped _ ((v,v') :: vvs)); repeat iSplit; eauto.
+    asimpl. iApply ('`IHHtyped ((v,v') :: vvs)); repeat iSplit; eauto.
     iApply interp_env_cons; iSplit; auto.
   Qed.
 
@@ -164,11 +171,12 @@ Section fundamental.
       (IHHtyped2 : Γ ⊨ e2 ≤log≤ e2' : τ1) :
     Γ ⊨ stlc_mu.lang.App e1 e2 ≤log≤ App e1' e2' :  τ2.
   Proof.
-    iIntros (Δ vvs ρ ?) "#[Hρ HΓ]"; iIntros (K) "Hj /=".
+    iIntros (vvs ei') "#[Hρ HΓ]"; iIntros (K) "Hj /=".
     smart_wp_bind (stlc_mu.lang.AppLCtx (e2.[stlc_mu.typing.env_subst (vvs.*1)])) v v' "[Hv #Hiv]"
-      ('`IHHtyped1 _ _ _ (((AppLCtx (e2'.[env_subst (vvs.*2)]))) :: K)); cbn.
+      ('`IHHtyped1 _ _ (((AppLCtx (e2'.[env_subst (vvs.*2)]))) :: K)); cbn.
     smart_wp_bind (stlc_mu.lang.AppRCtx v) w w' "[Hw #Hiw]"
-                  ('`IHHtyped2 _ _ _ ((AppRCtx v') :: K)); cbn.
+                  ('`IHHtyped2 _ _ ((AppRCtx v') :: K)); cbn.
+    rewrite interp_rw_TArrow.
     iApply ("Hiv" $! (w, w') with "Hiw"); simpl; eauto.
   Qed.
 
@@ -176,34 +184,31 @@ Section fundamental.
       (IHHtyped : Γ ⊨ e ≤log≤ e' : τ.[(TRec τ)/]) :
     Γ ⊨ stlc_mu.lang.Fold e ≤log≤ cast_calculus.lang.Fold e' : TRec τ.
   Proof.
-    iIntros (Δ vvs ρ ?) "#[Hρ HΓ]"; iIntros (K) "Hj /=".
+    iIntros (vvs ei') "#[Hρ HΓ]"; iIntros (K) "Hj /=".
     iApply (wp_bind (fill [stlc_mu.lang.FoldCtx])).
-    iApply (wp_wand with "[Hj]"). iApply ('`IHHtyped _ _ _ (FoldCtx :: K)). iFrame. auto.
+    iApply (wp_wand with "[Hj]"). iApply ('`IHHtyped _ _ (FoldCtx :: K)). iFrame. auto.
     iIntros (v); iDestruct 1 as (v') "[Hv #Hiv]".
     iApply wp_value.
     iExists (FoldV v'). iFrame "Hv".
-    rewrite fixpoint_interp_rec1_eq /= -interp_subst.
-    iAlways. iExists (_, _). eauto.
+    rewrite interp_rw_TRec.
+    iAlways. iExists _, _. eauto.
   Qed.
 
   Lemma bin_log_related_unfold Γ e e' τ
       (IHHtyped : Γ ⊨ e ≤log≤ e' : TRec τ) :
     Γ ⊨ stlc_mu.lang.Unfold e ≤log≤ Unfold e' : τ.[(TRec τ)/].
   Proof.
-    iIntros (Δ vvs ρ ?) "#[Hρ HΓ]"; iIntros (K) "Hj /=".
+    iIntros (vvs ei') "#[Hρ HΓ]"; iIntros (K) "Hj /=".
     iApply (wp_bind (fill [stlc_mu.lang.UnfoldCtx])).
-    iApply (wp_wand with "[Hj]"). iApply ('`IHHtyped _ _ _ (UnfoldCtx :: K)). iFrame. auto.
+    iApply (wp_wand with "[Hj]"). iApply ('`IHHtyped _ _ (UnfoldCtx :: K)). iFrame. auto.
     iIntros (v). iDestruct 1 as (v') "[Hw #Hiw]".
     simpl.
-    rewrite /= fixpoint_interp_rec1_eq /=.
-    change (fixpoint _) with (interp (TRec τ) Δ).
-    iDestruct "Hiw" as ([w w']) "#[% Hiz]"; simplify_eq/=.
+    rewrite interp_rw_TRec.
+    iDestruct "Hiw" as (w w') "#[% Hiz]"; simplify_eq/=.
     iMod (step_Fold _ _ K (of_val w') with "[-]") as "Hz"; eauto.
     iApply wp_pure_step_later; cbn; auto.
-    iNext. iApply wp_value; auto. iExists _; iFrame "Hz".
-      by rewrite -interp_subst.
+    iNext. iApply wp_value; auto.
   Qed.
-
 
 
 End fundamental.
