theories/stlc_mu/lang.v
@@ -193,3 +193,5 @@ Hint Extern 10 (AsVal _) =>
 
 Definition Halts (e : expr) :=
   ∃ v, rtc erased_step ([e], tt) ([of_val v], tt).
+
+Definition hack K : @LanguageCtx ectx_lang (fill K) := (ectx_lang_ctx K).
